big proof on or properity almost done (need to prove my_prefix_refl)

code/coq/det11.v
@@ -6,6 +6,24 @@ From det Require Import interpreter.
 From det Require Import aux.
 
 Definition g2a g := match g with Goal _ a => a end.
+Definition g2p g := match g with Goal g _ => g end.
+
+Definition make_empty_alts g := match g with Goal g _ => Goal g [::] end.
+Lemma save_alt_cons {a g1 gl l}: save_alt a (g1 :: gl) l = Goal g1 a :: save_alt a gl l.
+Proof. by []. Qed.
+Lemma more_alt_cons {a x xs tl} : more_alt a (x::xs) tl = save_alt a x tl :: more_alt a xs tl.
+Proof. by []. Qed.
+Lemma more_alt_empty_alts bs xs: more_alt [::] bs xs = [seq (save_alt [::] b xs) | b <- bs].
+Proof. unfold more_alt. by rewrite cats0. Qed.
+Lemma more_alt_empty_gl a xs: more_alt a [::] xs = a. auto. Qed.
+Lemma more_alt_empty {ys alts l}: more_alt ys alts l = [::] -> ys = [::].
+Proof. case: ys alts  => // la' l' alts.
+  unfold more_alt.
+  move=> H.
+  have:= (erefl (@size ((seq goal)) [::])).
+  rewrite -{1}H.
+  rewrite size_cat /= addnS //.
+Qed.
 
 Lemma map_cat_deep {T:Type} {R:Type} l gs:
   forall (P:T -> R),
@@ -17,38 +35,39 @@ Qed.
 
 (* Definition functional_prog' p :=
   forall n r g a, run p n g a = r -> r = None \/ r = Some a. *)
+Section Functionality.
+  Definition functional_prog p :=
+    forall n r g, run p n (not_alt_goal g) [::] = r -> r = None \/ r = Some [::].
 
-Definition functional_prog p :=
-  forall n r g, run p n (not_alt_goal g) [::] = r -> r = None \/ r = Some [::].
+  Definition functional_pred p f :=
+    forall n r, run p n [:: Goal (call f) [::]] [::] = r -> r = None \/ r = Some [::].
 
-Definition functional_pred p f :=
-  forall n r, run p n [:: Goal (call f) [::]] [::] = r -> r = None \/ r = Some [::].
+  Definition functional_goal p g :=
+    forall n r, run p n (not_alt_goal g) [::] = r -> r = None \/ r = Some [::].
 
-Definition functional_goal p g :=
-  forall n r, run p n (not_alt_goal g) [::] = r -> r = None \/ r = Some [::].
+  Definition functional_goal' p g :=
+    forall n r, run p n (not_alt_goal g) [::] = r -> r = Some [::].
 
-Definition functional_goal' p g :=
-  forall n r, run p n (not_alt_goal g) [::] = r -> r = Some [::].
-
-Lemma functional_neck_cut_all:
-  forall p, functional_prog (neck_cut_all p).
-Proof.
-  move=> prog n.
-  elim: n => /=.
-  - move=> r _ <-; auto.
-  - move=> n IH [sol|]; auto.
-    move=> [|[|p] gs] /=; auto.
-    + apply IH.
-    + simpl; unfold neck_cut_all.
-      destruct (prog p) as [|s] eqn:?; auto.
-      simpl; fold_neck_cut_all prog.
-      destruct n; auto.
-      move => /= H.
-      apply pumping1 in H.
-      specialize (IH (Some sol) (s ++ gs)).
-      rewrite <-map_cat in H.
-      now apply IH.
-Qed.
+  Lemma functional_neck_cut_all:
+    forall p, functional_prog (neck_cut_all p).
+  Proof.
+    move=> prog n.
+    elim: n => /=.
+    - move=> r _ <-; auto.
+    - move=> n IH [sol|]; auto.
+      move=> [|[|p] gs] /=; auto.
+      + apply IH.
+      + simpl; unfold neck_cut_all.
+        destruct (prog p) as [|s] eqn:?; auto.
+        simpl; fold_neck_cut_all prog.
+        destruct n; auto.
+        move => /= H.
+        apply pumping1 in H.
+        specialize (IH (Some sol) (s ++ gs)).
+        rewrite <-map_cat in H.
+        now apply IH.
+  Qed.
+End Functionality.
 
 Module Elpi.
   Definition success p g a :=
@@ -86,564 +105,307 @@ Definition build_goals ca gs := [seq Goal g ca | g <- gs].
 
 Arguments suffix {_}.
 Arguments prefix {_}.
-Fixpoint good_cut (l:list goal) (a: list alt) :=
-  match l with
-  | [::] => true
-  | Goal _ ca :: tl => suffix ca a && good_cut tl a
-  end. 
 
-Fixpoint good_levels (l:list alt) :=
-  match l with
-  | [::] => true
-  | x :: xs => good_cut x xs && good_levels xs
-  end.
+Section good_cut_and_level.
+
+  Inductive good_cut1 : list goal -> list alt -> Prop :=
+    | good_cut_nil a : good_cut1 [::] a
+    | good_cut_con g ca tl a : 
+      good_levels1 (tl :: ca) -> 
+        suffix ca a -> 
+          good_cut1 tl a -> 
+            good_cut1 (Goal g ca :: tl) a
+
+  with good_levels1 : list alt -> Prop :=
+    | good_levels1_nil : good_levels1 [::]
+    | good_levels1_con x xs: good_cut1 x xs -> good_levels1 xs -> good_levels1 (x::xs).
+
+  Lemma good_lvl1_cat {l1 l2} : 
+    good_levels1 (l1++l2) -> good_levels1 l2.
+  Proof.  
+    elim: l1 => //= x xs IH.
+    inversion 1; subst; auto.
+  Qed.
+
+  Lemma good_lvl1_suffix {ca} {a}: suffix ca a -> good_levels1 a -> good_levels1 ca.
+  Proof. move => /suffixP [x] -> /good_lvl1_cat //. Qed.
+
+  Lemma good_cut1_more_alt {gs tl a tl'}:
+    good_cut1 tl a -> good_cut1 tl (more_alt a gs tl').
+  Proof.
+    revert gs a tl'.
+    unfold more_alt, save_alt.
+    elim: tl => //=; try constructor.
+    move=> [g ca] tl IH gs a tl'.
+    inversion 1; subst.
+    apply good_cut_con => //.
+      now apply suffix_catr.
+    eapply IH; auto.
+  Qed.
+
+  Lemma good_cut1_save_alt {a g1 tl}:
+    good_cut1 tl a -> good_levels1 a -> good_cut1 (save_alt a g1 tl) a.
+  Proof.
+    elim: g1 => //= p L + GC GL => /(_ GC GL) IH.
+    rewrite save_alt_cons.
+    apply: good_cut_con => //; rewrite ?suffix_refl //.
+    apply: good_levels1_con => //.
+  Qed.
+
+  Lemma good_cut1_save_alt_more_alt {a b bs gl}:
+    good_cut1 gl a -> good_levels1 a -> good_cut1 (save_alt a b gl) (more_alt a bs gl).
+  Proof. apply: (fun x y => good_cut1_more_alt (good_cut1_save_alt x y)). Qed.
+
+  Lemma good_lvl1_more_alt {a gs tl}:
+    good_levels1 a -> good_cut1 tl a -> good_levels1 (more_alt a gs tl).
+  Proof.
+    elim: gs a tl => // gs0 gs IH a tl GL GC.
+    rewrite more_alt_cons.
+    constructor; auto.
+    by apply good_cut1_save_alt_more_alt.
+  Qed.
+
+  Lemma good_lvl1_save_alt_more_alt {a b bs gl}:
+    good_levels1 a -> good_cut1 gl a ->
+    good_levels1 (save_alt a b gl :: more_alt a bs gl).
+  Proof.
+    move=> H1 H2.
+    constructor.
+      by apply good_cut1_save_alt_more_alt.
+    by apply good_lvl1_more_alt.
+  Qed.
+
+  Lemma good_cut1_empty l : good_cut1 [seq make_empty_alts x | x <- l] [::].
+  Proof. by elim: l => /= [|[] a IH]; repeat constructor. Qed.
+
+  Lemma save_alt_with_make_empty_alt {a g1 tl}:
+    [seq make_empty_alts i  | i <- save_alt a g1 tl] = (save_alt [::] g1 [seq make_empty_alts i  | i <- tl]).
+  Proof. by elim: g1 => //= g1 gl IH /=; rewrite save_alt_cons IH. Qed.
+
+End good_cut_and_level.
 
 Inductive nur' (p: bodiesT) : list goal -> list alt -> (list alt) -> Prop :=
 | Stop a : nur' [::] a a
-| Cut a (ca:list alt) r gl : good_cut gl ca -> nur' gl ca r -> nur' [::Goal cut ca & gl] a r
+| Cut a (ca:list alt) r gl : good_cut1 gl ca -> nur' gl ca r -> nur' [::Goal cut ca & gl] a r
 | Fail a g al r : nur' a al r -> nur' g (a :: al) r
 | Call {a ca f b bs gl r} : p f = [:: b & bs ] ->
   nur' (save_alt a b gl) (more_alt a bs gl) r -> nur' [::Goal (call f) ca & gl] a r.
 
-Lemma good_lvl_cat {l1 l2} : 
-  good_levels (l1++l2) -> good_levels l2.
-Proof.   by elim: l1 => //= x xs IH /andP[_ /IH].  Qed.
 
-Lemma good_lvl_suffix {ca} {a}: suffix ca a -> good_levels a -> good_levels ca.
-Proof. by move => /suffixP [x] -> /good_lvl_cat /= . Qed.
+Section my_prefix.
 
-Lemma save_alt_cons {a g1 gl l}: save_alt a (g1 :: gl) l = Goal g1 a :: save_alt a gl l.
-Proof. by []. Qed.
+  Inductive forall2 {T R:Type} P : list T -> list R -> Prop := 
+    | forall2_nil : forall2 [::] [::]
+    | forall2_con {x xs y ys} : P x y -> forall2 xs ys -> forall2 (x::xs) (y::ys).
 
-Lemma more_alt_cons {a x xs tl} : more_alt a (x::xs) tl = save_alt a x tl :: more_alt a xs tl.
-Proof. by []. Qed.
+  Lemma forall2_refl {T : Type} (P : T -> T -> Prop) l : (forall x, P x x) -> forall2 P l l.
+  Proof. elim l; repeat constructor; auto. Qed.
 
-Lemma good_cut_more_alt {gs tl a tl'}:
-  good_cut tl a -> good_cut tl (more_alt a gs tl').
-Proof.
-  revert gs a tl'.
-  unfold more_alt, save_alt.
-  elim: tl => //= [[[|F]ca]tl] IH gs a tl'.
-    move=> /andP [H H1].
-    apply /andP; split.
-      now apply suffix_catr.
-    eapply IH; auto.
-  intros.
-  move /andP: H => [] S G.
-  apply /andP; constructor.
-    apply suffix_catr; auto.
-  eapply IH; auto.
-Qed.
+  (* Definition alt := seq goal. *)
+  (* Inductive goal := Goal (g : pred) (ca : list (list goal)). *)
+(*   Definition g2a g := match g with Goal _ a => a end.
+     Definition g2p g := match g with Goal g _ => g end. *)
+     
+  Definition forall2_alts P :=
+    forall2 (fun x y : goal => g2p x = g2p y /\ P (g2a x) (g2a y)).
 
-Lemma good_cut_save_alt {a g1 tl}:
-  good_cut tl a -> good_cut (save_alt a g1 tl) a.
-Proof.
-  elim: g1 => //= _ L + GC.
-  move => /(_ GC).
-  by rewrite suffix_refl.
-Qed.
+  Lemma forall2_alts_refl {P} l : (forall x, P x x) -> forall2  (fun x y : goal => g2p x = g2p y /\ P (g2a x) (g2a y)) l l.
+  Proof. elim l; repeat constructor; auto. Qed.
 
-Lemma good_cut_save_alt_more_alt {a b bs gl}:
-  good_cut gl a -> good_cut (save_alt a b gl) (more_alt a bs gl).
-Proof. move=> /(fun x => good_cut_more_alt (good_cut_save_alt x)) //. Qed.
+  Inductive my_prefix : seq alt -> seq alt -> Prop :=
+    | my_prefix_nil l : my_prefix [::] l
+    | my_prefix_con {x y xs ys} : 
+        forall2_alts my_prefix x y ->
+          my_prefix xs ys -> my_prefix (x :: xs) (y :: ys).
 
-Lemma good_cut_cat a: forall {b l}, good_cut a l -> good_cut b l -> good_cut (a ++ b) l.
-Proof. 
-  elim: a => //= [[[|F]ca]tl] IH b l /andP.
-    move=> [S_CA GC_TL] GC_B.
-    by apply /andP; auto.
-  move=> [S GTL] GB.
-  by apply /andP; constructor; auto.
-Qed.
+  Fixpoint my_prefix_refl_help (Px : forall x, forall2_alts my_prefix x x) (l : seq alt) : my_prefix l l :=
+    match l return my_prefix l l with
+    | [::] => my_prefix_nil [::]
+    | x :: xs => 
+         my_prefix_con (Px x) (my_prefix_refl_help Px xs)
+    end.
 
-Lemma good_cut_catr {a b c}:
-  good_cut (a ++ b) c -> good_cut b c.
-Proof. by elim: a => //= [] [] _ ca l IH /andP []. Qed.
-
-Lemma good_cut_catl {a b c}:
-  good_cut (a ++ b) c -> good_cut a c.
-Proof. elim: a => //= [] [] _ ca l IH /andP [] -> B; simpl; auto. Qed.
-
-Lemma good_lvl_more_alt {a gs tl}:
-  good_levels a -> good_cut tl a -> good_levels (more_alt a gs tl).
-Proof.
-  elim: gs a tl => // gs0 gs IH a tl GL GC.
-  rewrite more_alt_cons.
-  apply /andP; split; auto.
-  by apply good_cut_more_alt, good_cut_save_alt.
-Qed.
-
-(* prefix (more_alt alts bs0 (Goal (call f) ca :: l1)) (more_alt alts0 bs0 (Goal (call f) ca :: l1)) *)
-Lemma more_alt_empty {ys alts l}: more_alt ys alts l = [::] -> ys = [::].
-Proof. case: ys alts  => // la' l' alts.
-  unfold more_alt.
-  move=> H.
-  have:= (erefl (@size ((seq goal)) [::])).
-  rewrite -{1}H.
-  rewrite size_cat /= addnS //.
-Qed.
-
-Inductive forall2 {T R:Type} P : list T -> list R -> Prop := 
-  | forall2_nil : forall2 [::] [::]
-  | forall2_con {x xs y ys} : P x y -> forall2 xs ys -> forall2 (x::xs) (y::ys).
-
-Lemma forall2_refl {T : Type} (P : T -> T -> Prop) l : forall2 P l l.
-Proof. elim l. constructor. Abort. 
-
-(* Lemma forall2_cat {T: Type} (P: T->T->Prop) l1 l2: forall2 P l1 _ -> forall2 P l2 -> forall2 P (l1 ++ l2).  *)
-
-Definition g2p g := match g with Goal g _ => g end.
-Print all2.
-
-(* Fixpoint my_prefix l1 l2 {struct l1} :=
-  match l1, l2 with
-  | [::], _ => true
-  | x::xs, y::ys =>
-    my_prefix xs ys && all2 (fun '(Goal x a1) '(Goal y a2) => (x == y) && my_prefix a1 a2) x y
-  | _, _ => false
-  end.  *)
+  (* Fixpoint my_prefix_refl l :=
+    match l return my_prefix l l with
+    | nil => my_prefix_nil [::]
+    | x::xs => my_prefix_con ((forall2_alts_refl x (fun x => my_prefix_refl x)) : forall2_alts my_prefix x x) (my_prefix_refl xs)
+    end. *)
 
 
-Inductive my_prefix : seq alt -> seq alt -> Prop :=
-  | my_prefix_nil l : my_prefix [::] l
-  | my_prefix_sam {x y xs ys} : 
-      forall2 (fun x y => g2p x = g2p y /\ my_prefix (g2a x) (g2a y)) x y ->
-        my_prefix xs ys -> my_prefix (x :: xs) (y :: ys).
+  Lemma my_prefix_refl l: my_prefix l l.
+  Proof. 
+      have X := (my_prefix_refl_help).
+      have Y := forall2_refl (fun x y : goal => g2p x = g2p y /\ my_prefix (g2a x) (g2a y)).
+      induction l.
+        constructor.
+      constructor; auto.
+      (* Print and. *)
+      (* pose x:= 
+        fix f l :=
+          match l return (forall2_alts my_prefix l l) with
+          | nil => forall2_nil f
+          | x :: xs => Y x (conj erefl (fun y => X (f x) y))
+          end. *)
+        
+      apply Y.
+      constructor; auto.
+      apply X.
+      intro.
+      apply Y.
+      constructor; auto.
+      apply X.
+      intro.
+      apply Y.
+      constructor; auto.
+      apply X.
+      intro.
+      apply Y.
+      constructor; auto.
+      apply X.
+      intro.
+      apply Y.
+      constructor; auto.
+      apply X.
 
 
-
-Lemma my_prefix_refl l : my_prefix l l.
-Proof. 
-  elim l; constructor; auto.
-  elim a.
-  constructor.
-  intros.
-  constructor.
-  split.
-  auto.
-Abort.
-
-Lemma my_prefix_nil_ra {l}: my_prefix l [::] -> l = [::].
-Proof.
-  remember [::].
-  induction 1; try by [].
-Qed.
-
-Lemma my_prefix_cat {a b c d bs}: my_prefix a b -> forall2 (fun x y => g2p x = g2p y /\ my_prefix (g2a x) (g2a y)) c d -> my_prefix (more_alt a bs c) (more_alt b bs d).
-Proof.
   Admitted.
+      
 
-Lemma my_prefix_save_alt {gl ys a alts1 b}:
-  my_prefix a alts1 -> 
-  forall2 (fun x y : goal => g2p x = g2p y /\ my_prefix (g2a x) (g2a y)) gl ys ->
-  forall2 (fun x y : goal => g2p x = g2p y /\ my_prefix (g2a x) (g2a y)) (save_alt a b gl) (save_alt alts1 b ys).
-Admitted.
+  (* Lemma my_prefix_refl l : my_prefix l l.
+  Proof.
+    induction l; repeat constructor; auto.
+    eapply forall2_refl; constructor; auto.
 
+  Admitted. *)
 
-Lemma prefix_cat {T:eqType} (common: seq T) l1 l2: prefix l1 l2 -> prefix (common ++ l1) (common ++ l2).
-Proof. elim: common => //= c cs IH H; rewrite eqxx; auto. Qed.
+  Lemma forall2_my_prefix_refl g: forall2_alts my_prefix g g.
+  Proof. apply forall2_refl; split; auto; apply my_prefix_refl. Qed.
 
-Definition prefix_goal :=
-   (fun g1 g2 =>
-    match g1, g2 with
-    | Goal g ca, Goal g' ca' => 
-      g = g' /\ my_prefix ca ca' 
-    end).
+  Lemma my_prefix_nilr {l}: my_prefix l [::] -> l = [::].
+  Proof. by remember [::]; induction 1. Qed.
+
+  Lemma forall2_alts_my_prefix_save_alt {b gl ys a ALTS}:
+    my_prefix a ALTS -> forall2_alts my_prefix gl ys -> 
+      forall2_alts my_prefix (save_alt a b gl) (save_alt ALTS b ys).
+  Proof.
+    elim: b => //.
+    move=> p ca + A B  => /(_ A B) IH.
+    apply: forall2_con => //.
+  Qed.
+
+  Lemma my_prefix_more_alt {a b c d bs}: 
+    my_prefix a b -> forall2_alts my_prefix c d -> my_prefix (more_alt a bs c) (more_alt b bs d).
+  Proof.
+    elim bs => // x xs IH H1 H2.
+    move: IH => /(_ H1 H2) IH.
+    rewrite !more_alt_cons.
+    constructor.
+      by apply forall2_alts_my_prefix_save_alt.
+    by[].
+  Qed.
+
+  Lemma prefix_cat {T:eqType} (common: seq T) l1 l2: prefix l1 l2 -> prefix (common ++ l1) (common ++ l2).
+  Proof. elim: common => //= c cs IH H; rewrite eqxx; auto. Qed.
+
+End my_prefix.
 
 Lemma weaken_success' {prog alts g1 sol}:
   nur' prog g1 alts sol -> 
-  good_cut g1 alts -> good_levels alts -> 
+  good_levels1 (g1::alts) -> 
 
-  forall G1 alts1,
-    forall2 (fun x y => g2p x = g2p y /\ my_prefix (g2a x) (g2a y)) g1 G1 ->
-      good_cut G1 alts1 -> good_levels alts1 ->
-        my_prefix alts alts1 -> 
-          exists sol', nur' prog G1 alts1 sol'.
+  forall G1 ALTS,
+    forall2_alts my_prefix g1 G1 ->
+      good_levels1 (G1 :: ALTS) ->
+        my_prefix (g1 :: alts) (G1 :: ALTS) ->
+          exists sol', nur' prog G1 ALTS sol'.
 Proof.
   elim.
-  + inversion 3; subst.
+  + inversion 2; subst.
     repeat econstructor.
-  + move=> a ca r gl GCGL NUR IH GC GL G1 alts1.
-    inversion 1; subst; clear H.
-    destruct y.
-    simpl in H2; destruct H2; subst.
-    repeat econstructor; auto.
-      admit.
-    move: IH => /(_ _ _ _ _ H4 _ _ H0).
-    admit.
-  + move=> a g al r NUR IH.
-    move=> GCG GLAAL G1.
-    inversion 4; subst.
-    eexists. apply Fail.
+  
+  + move=> a ca r gl GCH NUR IH // GL G1 ALTS H.
+    inversion H as [|X Y [G1_p G1_ca] G1_gl [MP_g2p MP] F2].
+    simpl in MP_g2p, MP; subst; clear H.
+    move=> H; inversion H; subst; clear H.
+    inversion H2; subst; clear H2.
+    move=> PREF_a.
+    inversion PREF_a as [|???? F21 MP1]; subst ; clear PREF_a.
+    inversion F21 as [|???? [A B] _]; simpl in A; subst; clear F21 A.
+    simpl in *.
 
-    move: IH => /(_ _ _ _ _ H5 _ _ H7).
-    admit.
-  + move=> a ca f b bs gl r PF NUR IH.
-    move=> GC GL G1 alts1.
-    inversion 1; subst; clear H.
-    destruct y.
-    simpl in H2.
-    destruct H2; subst.
-    move=> GC11 GL11 PREF.
-    eexists. apply: Call PF _.
-    set (G1:= save_alt alts1 b ys).
-    set (alts':= more_alt alts1 bs ys).
-    have FF: forall2 (fun x y : goal => g2p x = g2p y /\ my_prefix (g2a x) (g2a y)) (save_alt a b gl) G1.
-      unfold G1.
-      now apply my_prefix_save_alt.
+    have GL_gl_ca: good_levels1 (gl :: ca).
+      constructor; auto.
+      inversion GL; subst.
+      inversion H1; subst.
+      by inversion H8; subst.
 
-    have HH: my_prefix (more_alt a bs gl) alts' .
-      unfold alts'.
-      by apply my_prefix_cat.
-    
-    move: IH => /(_ _ _ G1 alts' FF _ _ HH).
-    admit.
-Admitted.
+    have GL_ys_ca: good_levels1 (G1_gl :: G1_ca).
+      1:{
+        constructor.
+        inversion H4; subst; auto.
+        by epose proof (good_lvl1_suffix H6 H3).
+      }
 
-(* Lemma weaken_success' {prog a b bs gl sol}:
-  nur' prog (save_alt a b gl) (more_alt a bs gl) sol -> 
-  forall alts,
-    good_cut gl a -> good_levels a -> good_levels (gl::alts) ->
-      my_prefix a alts 
-      -> exists sol', nur' prog (save_alt alts b gl) (more_alt alts bs gl) sol'.
-Proof.
+    have GG: my_prefix (gl :: ca) (G1_gl :: G1_ca) by apply: my_prefix_con.
 
-Lemma weaken_success' {prog a b bs gl sol}:
-  nur' prog (save_alt a b gl) (more_alt a bs gl) sol -> 
-  forall alts,
-    good_cut gl a -> good_levels a -> good_levels (gl::alts) ->
-      my_prefix a alts 
-      -> exists sol', nur' prog (save_alt alts b gl) (more_alt alts bs gl) sol'.
-Proof.
-  move=> NUR alts GC GL1 GL2 PREF.
-  have: my_prefix (more_alt a bs gl) ((more_alt alts bs gl)).
-  by constructor.
-  remember (save_alt a b gl).
-  remember (more_alt a bs gl).
-  move=> NUR.
-  elim: NUR a b bs gl Heql Heql0 => /=.
-  + move=> aS a [] bs [] //=; repeat econstructor.
-  + move=> a ca r gl GCGL NUR IH alts [|bhd btl] // bs.
-      move=> [|glhd gls] //= [] H1 H2 H3; subst.
-      move=> alts' /andP [SCA GCGLS] GLALTS GLALTS'.
-      unfold save_alt; simpl.
-      exists r; eapply Cut; auto.
-    move=> gl' [] H1 H2 H3 H4; subst.
-    move: IH => /(_ alts btl [::] gl' erefl erefl) => IH.
-    move=> alts' A B C D.
-    move : IH => /(_ _ A B C D) [sol' IH].
-    rewrite save_alt_cons.
-    exists sol'; eapply Cut, IH.
-    apply good_cut_save_alt.
-    by move: C => /andP [].
-  + move=> a g al r NUR IH alts b.
-    move=> [|bshd bstl].
-      case: alts => // x xs gl' ? [] ? ?; subst.
-      move=> [] // a l1 GC /=.
-        move=> /my_prefix_nil_ra //.
-      move=> /andP [GCAXS GLXS] /= /andP [] GC_GL' /andP [GC_A GL_L1].
-      inversion 1; subst.
-        move: IH => /(_ xs [::] [::] a erefl erefl l1 GCAXS GLXS _ H1).
-        rewrite GC_A GL_L1 => /(_ isT) [{}sol IH].
-        by exists sol; apply Fail.
-      rewrite H1.
-      unfold more_alt; simpl.
-      (* eexists.
-      eapply Fail. *)
-      admit.
-      (* move: IH => /(_ _ [::] [::] a _ _ l1).
+    move: IH => /(_ GL_gl_ca G1_gl G1_ca F2 GL_ys_ca GG) [{}sol IH].
+    inversion GL_ys_ca; subst.
+    exists sol; apply: Cut H1 IH.
 
-      rewrite more_alt_cons.
+  + move=> a g al r NUR IH GL G1 ALTS F2 GL_G1.
+    inversion 1; subst; inversion H5; subst.
+    inversion H; subst; clear H.
 
-      move: IH => /(_ _ b [::] gl' _ _ (more_alt ys alts l2)) => /(_ (more_alt xs0 alts l2)). *)
-    move=> gl ?; subst.
-    rewrite more_alt_cons => [] [] ? ?; subst.
-    intros.
-    rewrite more_alt_cons.
-    move: IH => /(_ alts bshd bstl gl erefl erefl _ H H0 H1 H2) [{}sol IH].
+    have GL_a_al: good_levels1 (a :: al) by inversion GL; subst.
+    have GL_y_ys: good_levels1 (y :: ys) by inversion GL_G1; subst.
+
+    move: IH => /(_ GL_a_al y ys H2 GL_y_ys H5) [{}sol IH].
     by exists sol; apply Fail.
-  + move=> a ca f b bs gl r PF NUR IH alts [|bshd bstl] bs0.
-      move=> [] // a0 l1 [] ? ? ? /= alts0; subst.
-      move=> /andP [SCA0 GCL1 GLA] /andP [/andP []] A B C D.
-      set (more_alt alts bs0 (Goal (call f) ca :: l1)) as XX.
-      have AA: good_cut l1 XX.
-        now apply good_cut_more_alt.
-      have BB: good_levels XX.
-        apply good_lvl_more_alt; auto; simpl.
-        by rewrite SCA0 GCL1. 
-      set (more_alt alts0 bs0 (Goal (call f) ca :: l1)) as YY.
+  
+  + move=> a ca f b bs gl r PF NUR IH /= GL G1 ALTS F2 GL_G1_ALTS MP.
+    inversion MP; subst; clear MP.
+    inversion H2; subst; clear H2.
+    simpl in H1; destruct H1; simpl in *.
+    inversion F2; subst; simpl in *; clear F2.
+    clear H5.
+    destruct y; simpl in *; subst.
+    destruct H6; clear H.
+    inversion GL_G1_ALTS; clear GL_G1_ALTS; subst; inversion H3; subst; clear H3.
+    inversion GL; clear GL; subst; inversion H3; subst; clear H3.
+    have GL_SA_MA: good_levels1 (save_alt a b gl :: more_alt a bs gl).
+      by apply good_lvl1_save_alt_more_alt.
+    have F2': forall2_alts my_prefix (save_alt a b gl) (save_alt ALTS b ys).
+      by apply forall2_alts_my_prefix_save_alt.
+    have GL': good_levels1 (save_alt ALTS b ys :: more_alt ALTS bs ys).
+      by apply good_lvl1_save_alt_more_alt.
+    have MP': my_prefix (save_alt a b gl :: more_alt a bs gl) (save_alt ALTS b ys :: more_alt ALTS bs ys).
+      1: {
+        constructor; auto.
+        apply my_prefix_more_alt; auto.
+      }
 
-      have DD: good_cut l1 YY && good_levels YY.
-        have DD1: good_cut l1 YY.
-          unfold YY.
-          apply good_cut_more_alt.
-          by rewrite B.
-        have DD2: good_levels YY.
-          unfold YY.
-          apply good_lvl_more_alt; auto.
-          simpl.
-          by rewrite A B.
-        by rewrite DD1 DD2.
-      have EE: (my_prefix XX YY).
-        unfold XX, YY.
-        by constructor.
-      move: IH => /(_ _ _ _ _ erefl erefl YY AA BB DD EE) [{}sol IH].
-      by exists sol; apply: Call PF _.
-    move=> gl0 [] ? ? ? ? //; subst.
-    intros.
-    rewrite save_alt_cons.
-
-    have AA: (good_cut ([seq Goal x alts  | x <- bstl] ++ gl0) (more_alt alts bs0 gl0)).
-      by apply good_cut_save_alt_more_alt.
-    have BB: good_levels (more_alt alts bs0 gl0).
-      by apply good_lvl_more_alt.
-
-      
-  (* exists sol; apply: Call PF _.  *)
-    (* DA QUI *)
-    have KK : save_alt (more_alt alts bs0 gl0) b ([seq Goal x alts  | x <- bstl] ++ gl0) = save_alt (more_alt alts0 bs0 gl0) b (save_alt alts0 bstl gl0).
-      (* f_equal; auto. *)
-      (* unfold save_alt at 3. *)
-      admit.
-    have JJ : more_alt (more_alt alts bs0 gl0) bs ([seq Goal x alts  | x <- bstl] ++ gl0) = more_alt (more_alt alts0 bs0 gl0) bs (save_alt alts0 bstl gl0).
-      admit.
-    move: IH => /(_ _ b _ (save_alt alts0 bstl gl0) KK JJ (more_alt alts0 bs0 gl0)) .
-    move: H1 => /andP [] A B.
-    have TT: good_cut (save_alt alts0 bstl gl0) (more_alt alts0 bs0 gl0).
-      by apply good_cut_save_alt_more_alt.
-    have D: good_levels (more_alt alts0 bs0 gl0).
-      apply good_lvl_more_alt; auto.
-
-    rewrite D TT => /(_ isT isT isT (my_prefix_refl _)) [{}sol IH].
-    exists sol; apply: Call PF IH.
-    (* A QUI *)
-
-    eapply my_prefix_moa in H2.
-    move: H1 => /andP [] A B.
-    move: IH => /(_ _ _ _ _ erefl erefl _ AA BB) => /(_ (more_alt alts0 bs0 gl0) _ H2).
-    have BA: good_cut ([seq Goal x alts  | x <- bstl] ++ gl0) (more_alt alts0 bs0 gl0).
-      apply good_cut_cat.
-      2:{ by apply good_cut_more_alt. }
-      admit.
-
-    rewrite BA (good_lvl_more_alt B A) => /(_ isT) [{}sol IH].
-    eexists.
-    apply: Call PF _.
-    apply IH.
-
-Admitted.
-
-
-Lemma weaken_success {prog g a r}:
-  nur' prog g a r -> good_levels (g::a) -> forall a1, 
-     my_prefix a a1 -> good_levels (g::a1) ->
-      exists r1, nur' prog g a1 r1.
-Proof.
-  move=> NUR.
-  elim: NUR => /=.
-  + repeat econstructor.
-  + move=> {}a ca {}r gl GC_GL NUR' IH /andP [/andP [SCA GCGL] GLA] aext PREF.
-    have : good_cut gl ca && good_levels ca.
-      rewrite (good_lvl_suffix SCA GLA).
-      by rewrite GC_GL.
-    have GG: good_cut gl ca && good_levels ca.
-      by rewrite GC_GL (good_lvl_suffix SCA GLA).
-    move=> /IH /(_ _ (my_prefix_refl ca) GG) [sol {IH}].
-    by exists sol; repeat constructor.
-  + move=> {}a {}g {}al {}r NUR IH /and3P [GC_G GC_A GL_AL] [|aext1 aext] + /andP [GC_G' GC_aext] //.
-      move=> /my_prefix_nil_r => /(_ (g)) [] [|aa aas] // [] ? ?; subst.
-        admit.
-      
-    have: good_cut (save_alt [::] aa (g)) ([seq save_alt [::] b (g)  | b <- aas] ++ [::]) &&
-good_levels ([seq save_alt [::] b (g)  | b <- aas] ++ [::]) by admit.
-
-    move=> GCAAL.
-    move: IH => /(_ GCAAL).
-    unfold save_alt.
-     aext). PREF GC_aext) [x IH].
-    by exists x; apply Fail.
-  + move=> {}a ca f b bs gl {}r PF NUR IH /andP [/andP []] HK1 HK2 HK3.
-    have IH1: good_cut (save_alt a b gl) (more_alt a bs gl) && good_levels (more_alt a bs gl).
-      by rewrite good_cut_save_alt_more_alt ?good_lvl_more_alt //.
-    move: IH => /(_ IH1 (more_alt a bs gl) ) /(_ (prefix_refl _) IH1) [sol HSol] alts PREF /andP [/andP] [] A B C.
-
-    epose proof (weaken_success' HSol _ HK2 HK3 _ PREF) as [sol'].
-    (* epose proof (weaken_success' HSol _ HK2 HK3 PREF) as [sol']. *)
-    by eexists sol'; apply: Call PF _.
-    Unshelve.
-    simpl.
-    by rewrite B C.
-Qed. *)
+    move: IH => /(_ GL_SA_MA (save_alt ALTS b ys) (more_alt ALTS bs ys) F2' GL' MP') [{}sol IH].
+    eexists sol. apply: Call PF IH.
+Qed.
 
 Lemma weaken_success_nil {prog g a r}:
-  good_levels (g::a) ->
-    nur' prog g [::] r -> good_levels (g::[::]) ->
+  good_levels1 (g::a) ->
+    nur' prog g [::] r -> good_levels1 (g::[::]) ->
     exists r1, nur' prog g a r1.
-Proof. move=> GLGA NUR GLG .
-
-  epose proof (weaken_success' NUR _ isT g a).
-
- => /weaken_success /(_ GLG a (prefix0s _) GLGA) //. Qed.
-
-Definition make_empty_alts g := match g with Goal g _ => Goal g [::] end.
-
-Lemma good_cut_empty l : good_cut [seq make_empty_alts x | x <- l] [::].
- by elim: l => //= -[f ? gl] IH /=.
+Proof.
+    move=> GLGA NUR GLG .
+    have MP: (my_prefix [::g] (g::a)).
+      repeat constructor.
+      by apply forall2_my_prefix_refl.
+    have [sol IH] := weaken_success' NUR GLG g a (forall2_my_prefix_refl _) GLGA MP.
+    by exists sol.
 Qed.
-
-Lemma save_alt_with_make_empty_alt {a g1 tl}:
-  [seq make_empty_alts i  | i <- save_alt a g1 tl] = (save_alt [::] g1 [seq make_empty_alts i  | i <- tl]).
-Proof.
-  elim: g1 => //= g1 gl IH /=.
-  by rewrite save_alt_cons IH.
-Qed.
-
-Definition less l1 l2 :=
-  forall p1 p2 s, p1 ++ s = l1 -> p2 ++ s = l2 -> forall e1 e2, e1 \in p1 -> e2 \in p2 -> suffix (g2a e1) (g2a e2).
-
-Lemma less_save_alt {x0 g1 tl f ca a} :
-  suffix ca a ->
-  less x0 ([seq Goal x a  | x <- g1] ++ tl) ->
-    less x0 (Goal (call f) ca :: tl).
-Proof.
-Abort.
-
-Lemma succeed_more_alts {prog sol g1 g2 alts}:
-  nur' prog g1 alts sol ->
-    less g1 g2 ->
-      nur' prog g2 alts sol.
-Abort.
-
-(* THIS IS WRONG: we can have (g::gs) = [[!,fail],[::]] 
-  the cut prevent the alternative to be used
-*)
-Lemma nur_empty_goal {prog g gs}:
-  good_levels (g::gs) ->
-  [::]  \in (g :: gs) ->
-    exists s, nur' prog g gs s.
-Proof.
-  revert gs.
-  elim: g => [|[] gtl] /=.
-    move=> gs; exists gs; constructor.
-  move=> ca l IH gs /andP [/andP [SIH  GC]] GS.
-  rewrite in_cons => /orP [] //= NGS.
-  have b': [::] \in l :: gs.
-    by rewrite in_cons NGS orbC.
-  have GC_GL: good_cut l gs && good_levels gs.
-    by apply /andP.
-  specialize (IH _ GC_GL b') as [].
-  destruct gtl.
-Abort.
-  
-  
-(* THIS IS NOT TRUE: if gs = [[!, fail], [true]]
-  the hyp is satisfied: there is a goal in gs which succeed (namely the second)
-  the conclusion is however wrong: run (!, fail) [true] can't succeed
- *)
-Lemma call_success {prog g' a s gs tl f}:
-  nur' prog g' [::] s ->
-    prog f = gs ->
-      g' \in [seq [seq make_empty_alts i  | i <- i]  | i <- [seq save_alt a b tl  | b <- gs]] ->
-        exists (s' : seq alt),
-          nur' prog (Goal (call f) [::] :: [seq make_empty_alts i  | i <- tl]) [::] s'.
-Proof.
-Abort.
-
-Definition siblings l1 l2 :=
-  match l1, l2 with 
-  | [::], _ | _, [::] => True
-  | Goal _ a::_, Goal _ b::_ => a = b 
-  end.
-
-Definition is_call x := match x with Goal cut _ => false | _ => true end.
-
-Definition all_same_level_before_have_not_cut (g:list goal) (l:list alt) :=
-  exists bef, 
-    prefix (rcons bef g) l /\
-      exists x, 
-        x \in bef /\ 
-          all is_call x.
-
-Lemma run_with_nil_and_all_is_call {prog g bef alts}:
-good_levels (g::alts) ->
-  prefix (rcons bef [::]) alts
-    -> all is_call g
-      -> all (all is_call) (bef)
-        -> exists s', nur' prog g alts s'.
-Proof.
-  revert g bef.
-  induction alts.
-    destruct bef; try by [].
-  destruct g as [|ghd gtl].
-    repeat econstructor.
-  destruct ghd as [[|F] ca].
-    by[].
-  destruct (prog F) as [|fhd ftl] eqn:PF.
-    (* here prog F has no solution: therefore call Fail *)
-    destruct bef as [|befhd bef]; simpl.
-      move=> /and3P [/andP [SCA GCCTLA] GCA] GLA /andP [/eqP HA PNil]; subst.
-      repeat econstructor.
-    move=> /and3P [/andP [SCA GCGTLA] GCA] GLA /andP [/eqP HL PBEF] AGTL /andP [AA AAB]; subst a; simpl in *.
-    have IHH: good_cut befhd alts && good_levels alts.
-      by apply /andP.
-    specialize (IHalts befhd bef IHH PBEF AA AAB) as [].
-    repeat econstructor; apply H.
-
-  (* here prog F has solution fhd ftl *)
-  move=> bef /= .
-Abort.
-
-
-Lemma run_with_nil_and_all_is_call' {prog alts tl x bef gs}:
-  prefix (rcons bef [::])
-    [seq [seq make_empty_alts i0  | i0 <- i] | i <- [seq save_alt alts b tl  | b <- gs]] 
-    -> x  = [seq make_empty_alts i  | i <- tl]
-      -> all is_call x
-        -> exists s' : seq alt,
-          nur' prog [seq make_empty_alts i  | i <- tl]
-          (more_alt [::] gs [seq make_empty_alts i  | i <- tl]) s'.   
-Proof. Abort.
-
-Lemma aa {prog g' s g1 gs a tl}:
-  good_cut tl a -> good_levels a ->
-  nur' prog g' [::] s ->
-    all_same_level_before_have_not_cut g' [seq [seq make_empty_alts i  | i <- i] | i <- [seq save_alt a b tl  | b <- g1 :: gs]] ->
-    (* g' \in [seq [seq make_empty_alts i  | i <- i] | i <- [seq save_alt a b tl  | b <- g1 :: gs]] -> *)
-      exists s',
-        nur' prog (save_alt [::] g1 [seq make_empty_alts i  | i <- tl]) (more_alt [::] gs [seq make_empty_alts i  | i <- tl]) s'.
-Proof.
-  remember [::].
-  move=> + + NUR.
-  move: Heql tl a g1 gs.
-  induction NUR; subst.
-  + 1:{
-    move=> -> tl alts g1 gs GC GL [bef [+ [x [+ IS_CALL]]]]; simpl in *.
-    destruct bef; try by [].
-    move=> /= /andP [/eqP H PREF]; subst.
-    rewrite in_cons => /orP [/eqP H| ]; subst.
-
-      erewrite save_alt_with_make_empty_alt in IS_CALL.
-      destruct g1.
-        destruct tl.
-          repeat econstructor.
-        rewrite <-@save_alt_with_make_empty_alt with (a:=[::]).
-        simpl.
-        destruct g; destruct g; try by [].
-        destruct (prog n) eqn:?.
-        destruct gs; simpl; unfold more_alt.
-        destruct bef; try by [].
-        simpl.
-        econstructor. 
-        apply Fail.
-
-        repeat econstructor.
-Abort.
 
 Lemma cons_cat {T:Type} {a b c}: (a:T)::b++c = ([::a]++b)++c. by []. Qed.
 
 Lemma cut_semantic {prog s g alts}:
     nur' prog g alts s ->
-      good_levels (g::alts) ->
+      good_levels1 (g::alts) ->
         exists g' s', g' \in (map (map make_empty_alts) (g :: alts)) 
           (*e tutti quelli che precedono g' e che sono dello stesso livello non hanno cut 
             o falliscono prima di raggiungere il cut*) 
@@ -652,51 +414,49 @@ Proof.
   elim => /=.
   - exists [::], [::]; repeat constructor; auto.
 
-  - move => a ca r gl GC H /= IH /= /andP [/andP [ H1 H2 ] H3].
-    have IH_p : good_cut gl ca && good_levels ca.
-      by rewrite (good_lvl_suffix H1) ?GC; auto.
-    case: (IH IH_p) => g' [s' [+ NUR]].
+  - move => a ca r gl GC H /= IH /= GL. 
+    inversion GL as [|gs alts' GC1 GL1 C]; subst; clear GL.
+    inversion GC1 as [| P CA TL ALTS GL2 SUFF GC2]; subst; clear GC1.
+    case: (IH GL2) => g' [s' [+ NUR]].
     rewrite in_cons => /orP; case.
     - move=> /eqP?; subst.
       exists (map make_empty_alts (Goal cut ca :: gl)), s'; constructor; auto.
         by rewrite inE eqxx.
-      by simpl; apply: Cut => //; apply: good_cut_empty.
+      by simpl; apply: Cut => //; apply: good_cut1_empty.
     - move=> g'_ca.
       exists g', s'.
       split; last by [].
       rewrite inE orbC.
-      case/suffixP: H1 => a' ->. 
+      case/suffixP: SUFF => a' ->. 
       by rewrite map_cat mem_cat g'_ca orbT.
 
-  - move=> g' gl al solution H + /and3P [] p p0 p1.
-    case; first by rewrite p0 p1.
-    move=> x [s' [IN NUR]].
-    exists x, s'.
-    split; last by [].
-    by rewrite in_cons IN orbT.
+  - move=> {}g gl al solution H + GL.
+    inversion GL as [|g' a2 GC1 GL1]; subst; clear GL.
+    move=> /(_ GL1) [g' [sol ]] [] IN NUR'.
+    exists g', sol; auto.
+    by rewrite in_cons IN orbC.
 
-  - move=> a ca f g1 gs tl r PF NUR + /andP [/andP [_ GC] GL].
-    rewrite (good_cut_more_alt (good_cut_save_alt GC)) (good_lvl_more_alt GL GC) => /(_ isT).
-    case=>[g'[s' [+ NUR']]].
+  - move=> a ca f g1 gs tl r PF NUR + GL.
+    inversion GL as [|gs' alts' GC1 GL1 C]; subst; clear GL.
+    inversion GC1 as [| P CA TL ALTS GL2 SUFF GC2]; subst; clear GC1.
+    have GL_SA_MA: good_levels1 (save_alt a g1 tl :: more_alt a gs tl) by apply good_lvl1_save_alt_more_alt.
+    move=> /(_ (good_lvl1_save_alt_more_alt GL1 GC2)) [g' [s' [+ NUR']]].
     unfold more_alt.
-    rewrite map_cat cons_cat mem_cat => /orP. case.
-    2:{ exists g', s'; constructor; auto. by rewrite in_cons b orbC. }
+    rewrite map_cat cons_cat mem_cat => /orP.
+    move=> [+|INA] //=.
+    2:{ exists g', s'; constructor; auto; by rewrite in_cons INA orbC. }
     simpl.
     rewrite <-map_cons.
     replace (save_alt a _ _ :: [seq _ | _ <- _]) with [seq save_alt a b tl | b <- g1 :: gs ] by auto.
-    rewrite /= in_cons => /orP GIN.
+
+    move=> IN_IMPL.
     exists ((Goal (call f) [::] :: [seq make_empty_alts i  | i <- tl])).
     
     set (empty_tl:= map make_empty_alts tl).
 
-    suffices: exists s, nur' prog (save_alt [::] g1 empty_tl) (more_alt [::] gs empty_tl) s.
-      move=> [sol' H'].
-      eexists; split; auto.
-      by rewrite in_cons eqxx /=.
-      apply: Call PF H'.
-    
-    have {}GIN: (g' = save_alt [::] (g1) (empty_tl) \/ g' \in [seq save_alt [::] b (empty_tl)  | b <- gs]).
-      move: GIN => [/eqP |] H.
+    have GR: (g' = save_alt [::] (g1) (empty_tl) \/ g' \in [seq save_alt [::] b (empty_tl)  | b <- gs]).
+      move: IN_IMPL.
+      rewrite /= in_cons => /orP [/eqP |] H.
       rewrite save_alt_with_make_empty_alt in H; auto.
       right.
       congr(g' \in _) : H.
@@ -704,57 +464,88 @@ Proof.
       rewrite -map_comp.
       apply: eq_map.
       move=> ? /=.
-      by erewrite save_alt_with_make_empty_alt.
-
-    have GL_G' : good_levels [:: g'].
-      destruct GIN; subst.
+      by rewrite save_alt_with_make_empty_alt.
+    
+    have GL_G' : good_levels1 [:: g'].
+      constructor.
+      destruct GR; subst.
         simpl.
         rewrite -(@save_alt_with_make_empty_alt [::]).
-        by rewrite good_cut_empty.
-      elim: gs H {PF NUR} => //=.
+        apply good_cut1_empty.
+      elim: gs H {PF NUR GL_SA_MA IN_IMPL} => //=.
       move=> x xs IH.
       rewrite in_cons => /orP [/eqP H |]; subst.
         rewrite -(@save_alt_with_make_empty_alt [::]).
-        by rewrite good_cut_empty.
+        apply good_cut1_empty.
       auto.
+      constructor.
+    rewrite in_cons eqxx /=.
 
-    have GL_G_TL: good_levels (g' :: more_alt [::] gs empty_tl).
-      simpl.
-      rewrite /= andbC /= in GL_G'.
-      rewrite good_cut_more_alt ?GL_G' //.
-      rewrite good_lvl_more_alt //.
-      by rewrite good_cut_empty.
+    have GL_G_TL: good_levels1 (g' :: more_alt [::] gs empty_tl).
+      constructor.
+      inversion GL_G'; subst.
+      by apply good_cut1_more_alt.
+      apply good_lvl1_more_alt.
+        constructor.
+      apply good_cut1_empty.
 
-    destruct GIN.
-     have {} NUR' := @weaken_success_nil _ _ (more_alt [::] gs empty_tl) _ GL_G_TL NUR' GL_G'.
-      destruct NUR'. 
-      eexists x.
-      by subst.
-    
+    case: GR => [EQ|IN].
+      subst.
+
+      have [sol {}NUR'] := @weaken_success_nil _ _ (more_alt [::] gs empty_tl) _ GL_G_TL NUR' GL_G'. 
+      eexists; split; auto.
+      apply: Call PF NUR'.
+
     suffices: exists s',  nur' prog (save_alt [::] g1 empty_tl) (more_alt [::] gs empty_tl) s'.
       move=> [sol' H'].
-      by eexists sol'.
+      eexists; split; auto.
+      apply: Call PF H'.
 
-    elim: gs  (save_alt [::] g1 empty_tl) H NUR' {NUR PF GL_G_TL} => [|x xs IH] //= G.
+    elim: gs  (save_alt [::] g1 empty_tl) IN NUR' {NUR PF GL_G_TL GL_SA_MA IN_IMPL} => [|x xs IH] //= G.
 
     rewrite in_cons => /orP [/eqP H | ].
-      move=> NUR.
-      have GL_G_TL: good_levels (g' :: more_alt [::] xs empty_tl).
-        simpl.
-        rewrite /= andbC /= in GL_G'.
-        rewrite good_cut_more_alt ?GL_G' //.
-        rewrite good_lvl_more_alt //.
-        by rewrite good_cut_empty.
+    move=> NUR.
+    have GL_G_TL: good_levels1 (g' :: more_alt [::] xs empty_tl).
+      1:{
+        subst.
+        apply good_lvl1_save_alt_more_alt.
+          constructor.
+        apply good_cut1_empty.
+      }
 
-      have [sol {}NUR] := @weaken_success_nil _ _ (more_alt [::] xs empty_tl) _ GL_G_TL NUR GL_G'.
-      exists sol.
-      rewrite more_alt_cons.
-      by apply Fail; subst.
-
+    have [sol {}NUR] := @weaken_success_nil _ _ (more_alt [::] xs empty_tl) _ GL_G_TL NUR GL_G'.
+    exists sol.
+    rewrite more_alt_cons.
+    apply Fail.
+    subst; apply NUR.
     move=> /IH IH' /IH' H.
     destruct (H (save_alt [::] x empty_tl)).
+    exists x0.
     rewrite more_alt_cons.
-    by exists x0; apply Fail.
+    apply Fail.
+    auto.
 Qed.
 
 Print Assumptions cut_semantic.
+
+Definition functional_goal'' p :=
+  forall g s, nur' p (map make_empty_alts g) [::] s -> s = [::].
+
+Lemma functional_goal_ p:
+  functional_goal'' (tail_cut_all p).
+Proof.
+  move=> g s H1.
+  remember (tail_cut_all p) as p'.
+  remember [::] as el.
+  remember (map make_empty_alts g) as mg.
+  elim: H1 g Heqel Heqmg => //=; subst.
+  + move=> a ca r gl GC NUR IH [|[gp gca] gs] ? //= [] ???; subst.
+    apply: IH erefl erefl.
+  + move=> a ca f b bs gl r PF NUR IH [|[gp gca] gs] //= ?[??]?; subst.
+    rewrite more_alt_empty_alts in IH.
+    erewrite <-save_alt_with_make_empty_alt in IH.
+    move: IH => /(_ (save_alt [::] b gs) _ erefl).
+
+
+
+
